<?xml version="1.0"?>
<rdf:RDF xmlns="http://www.iri.upc.edu/groups/perception/OCRA/ont/ocra_plan.owl#"
     xml:base="http://www.iri.upc.edu/groups/perception/OCRA/ont/ocra_plan.owl"
     xmlns:dc="http://purl.org/dc/elements/1.1/"
     xmlns:owl="http://www.w3.org/2002/07/owl#"
     xmlns:rdf="http://www.w3.org/1999/02/22-rdf-syntax-ns#"
     xmlns:xml="http://www.w3.org/XML/1998/namespace"
     xmlns:xsd="http://www.w3.org/2001/XMLSchema#"
     xmlns:rdfs="http://www.w3.org/2000/01/rdf-schema#">
    <owl:Ontology rdf:about="https://github.com/indigo-the-agent/aamas2024_submission709/2-ontology/ocra_plan.owl">
        <owl:imports rdf:resource="http://www.iri.upc.edu/groups/perception/OCRA/ont/ocra.owl"/>
        <rdfs:comment xml:lang="en">This (application) ontology includes concepts and relations commonly found in planning for robotics to support the use of the ontology for collaborative robotics and adaptation (OCRA) [1]. Specifically, the ontology models the knowledge about how different plans compare to each other. 


[1] Olivares-Alarcos, A., Foix, S., Borgo, S., &amp; Alenyà, G. (2022). OCRA–An ontology for collaborative robotics and adaptation. Computers in Industry, 138, 103627.</rdfs:comment>
    </owl:Ontology>
    


    <!-- 
    ///////////////////////////////////////////////////////////////////////////////////////
    //
    // Object Properties
    //
    ///////////////////////////////////////////////////////////////////////////////////////
     -->

    


    <!-- https://github.com/indigo-the-agent/aamas2024_submission709/2-ontology/ocra_plan.owl#grasps -->

    <owl:ObjectProperty rdf:about="https://github.com/indigo-the-agent/aamas2024_submission709/2-ontology/ocra_plan.owl#grasps">
        <rdfs:subPropertyOf rdf:resource="http://www.ontologydesignpatterns.org/ont/dul/DUL.owl#associatedWith"/>
        <owl:inverseOf rdf:resource="https://github.com/indigo-the-agent/aamas2024_submission709/2-ontology/ocra_plan.owl#isGraspedBy"/>
        <rdfs:domain rdf:resource="http://www.ontologydesignpatterns.org/ont/dul/DUL.owl#Agent"/>
        <rdfs:range rdf:resource="http://www.ontologydesignpatterns.org/ont/dul/DUL.owl#PhysicalObject"/>
        <rdfs:comment xml:lang="en">Property to capture the relation between an agent and a physical object grasped by the agent. 

This relation is meant to be used for physical objects only, thus it is not consider the case of &apos;grasping and idea&apos;. For example, one might use this relation to represent the fact that a robot is grasping a piece of cloth.</rdfs:comment>
        <rdfs:label xml:lang="en">grasps</rdfs:label>
    </owl:ObjectProperty>
    


    <!-- https://github.com/indigo-the-agent/aamas2024_submission709/2-ontology/ocra_plan.owl#hasBetterQualityValueThan -->

    <owl:ObjectProperty rdf:about="https://github.com/indigo-the-agent/aamas2024_submission709/2-ontology/ocra_plan.owl#hasBetterQualityValueThan">
        <rdfs:subPropertyOf rdf:resource="http://www.ontologydesignpatterns.org/ont/dul/DUL.owl#associatedWith"/>
        <owl:inverseOf rdf:resource="https://github.com/indigo-the-agent/aamas2024_submission709/2-ontology/ocra_plan.owl#hasWorseQualityValueThan"/>
        <rdfs:domain rdf:resource="http://www.ontologydesignpatterns.org/ont/dul/DUL.owl#Quality"/>
        <rdfs:range rdf:resource="http://www.ontologydesignpatterns.org/ont/dul/DUL.owl#Quality"/>
        <rdfs:comment xml:lang="en">Relation between two Qualities that indicates that one of the qualities has a better value than the other quality with respect to some criteria. 

Note that this ontology aims to model the result of comparing two qualities&apos; values, but it is out of the scope of the model to make any commitment regarding which is the criteria to compare the different values.</rdfs:comment>
        <rdfs:label xml:lang="en">has better quality value than</rdfs:label>
    </owl:ObjectProperty>
    


    <!-- https://github.com/indigo-the-agent/aamas2024_submission709/2-ontology/ocra_plan.owl#hasCost -->

    <owl:ObjectProperty rdf:about="https://github.com/indigo-the-agent/aamas2024_submission709/2-ontology/ocra_plan.owl#hasCost">
        <rdfs:subPropertyOf rdf:resource="http://www.ontologydesignpatterns.org/ont/dul/DUL.owl#hasQuality"/>
        <owl:inverseOf rdf:resource="https://github.com/indigo-the-agent/aamas2024_submission709/2-ontology/ocra_plan.owl#isCostOf"/>
        <rdfs:domain rdf:resource="http://www.ontologydesignpatterns.org/ont/dul/DUL.owl#Plan"/>
        <rdfs:range rdf:resource="http://www.ontologydesignpatterns.org/ont/dul/DUL.owl#Quality"/>
        <rdfs:comment xml:lang="en">Relation between a Plan and a Quality that indicates the cost of executing the plan.

One might think that this relation could be modeled as a Data property instead of using an Object property. However, data instances cannot act as subjects in triples, thus, it would not be possible to represent some desirable statements such as &apos;the cost of a plan is better/worse/equivalent to the cost of a nother plan&apos;. For this reason, the relation is modeled as an Object property and users will need to add the actual value using the data property &apos;has data value&apos;.  

Example of use: Px (instance of Plan) &apos;has cost&apos; Qx (instance of Quality) that &apos;has data value&apos; 85. 

It is recomended to use an unsigned real number for the econded value, thus, the cost would be zero or greater than zero.</rdfs:comment>
        <rdfs:label xml:lang="en">has cost</rdfs:label>
    </owl:ObjectProperty>
    


    <!-- https://github.com/indigo-the-agent/aamas2024_submission709/2-ontology/ocra_plan.owl#hasEquivalentQualityValueThan -->

    <owl:ObjectProperty rdf:about="https://github.com/indigo-the-agent/aamas2024_submission709/2-ontology/ocra_plan.owl#hasEquivalentQualityValueThan">
        <rdfs:subPropertyOf rdf:resource="http://www.ontologydesignpatterns.org/ont/dul/DUL.owl#associatedWith"/>
        <owl:inverseOf rdf:resource="https://github.com/indigo-the-agent/aamas2024_submission709/2-ontology/ocra_plan.owl#hasEquivalentQualityValueThan"/>
        <rdf:type rdf:resource="http://www.w3.org/2002/07/owl#SymmetricProperty"/>
        <rdfs:domain rdf:resource="http://www.ontologydesignpatterns.org/ont/dul/DUL.owl#Quality"/>
        <rdfs:range rdf:resource="http://www.ontologydesignpatterns.org/ont/dul/DUL.owl#Quality"/>
        <rdfs:comment xml:lang="en">Relation between two Qualities that indicates that both qualities have a equivalent value with respect to some criteria. 

Note that this ontology aims to model the result of comparing two qualities&apos; values, but it is out of the scope of the model to make any commitment regarding which is the criteria to compare the different values.</rdfs:comment>
        <rdfs:label xml:lang="en">has equivalent quality value than</rdfs:label>
    </owl:ObjectProperty>
    


    <!-- https://github.com/indigo-the-agent/aamas2024_submission709/2-ontology/ocra_plan.owl#hasExpectedMakespan -->

    <owl:ObjectProperty rdf:about="https://github.com/indigo-the-agent/aamas2024_submission709/2-ontology/ocra_plan.owl#hasExpectedMakespan">
        <rdfs:subPropertyOf rdf:resource="http://www.ontologydesignpatterns.org/ont/dul/DUL.owl#hasQuality"/>
        <owl:inverseOf rdf:resource="https://github.com/indigo-the-agent/aamas2024_submission709/2-ontology/ocra_plan.owl#isExpectedMakespanOf"/>
        <rdfs:domain rdf:resource="http://www.ontologydesignpatterns.org/ont/dul/DUL.owl#Plan"/>
        <rdfs:range rdf:resource="http://www.ontologydesignpatterns.org/ont/dul/DUL.owl#Quality"/>
        <rdfs:comment xml:lang="en">Relation between a Plan and a Quality that indicates the expected number of time units that will elapse from the start of the work described in the plan to the end.

One might think that this relation could be modeled as a Data property instead of using an Object property. However, data instances cannot act as subjects in triples, thus, it would not be possible to represent some desirable statements such as &apos;the makespan of a plan is better/worse/equivalent to the makespan of a nother plan&apos;. For this reason, the relation is modeled as an Object property and users will need to add the actual value using the data property &apos;has data value&apos;.  

Example of use: Px (instance of Plan) &apos;has expected makespan&apos; Qx (instance of Quality) that &apos;has data value&apos; 1600. 

It is recomended to use the International System of Units, thus, the encoded data value would be in seconds. However, users of this ontology might assert values in different units, as long as they specify it. For instance, they might add a subproperty of either this relation (&apos;has expected makespan in hours&apos; or the property &apos;has data value&apos; (&apos;has data value in hours&apos;).  this data property to indicate makespans using different units (e.g., hasExpectedMakespanInHours).</rdfs:comment>
        <rdfs:label xml:lang="en">has expected makespan</rdfs:label>
    </owl:ObjectProperty>
    


    <!-- https://github.com/indigo-the-agent/aamas2024_submission709/2-ontology/ocra_plan.owl#hasNumberOfTasks -->

    <owl:ObjectProperty rdf:about="https://github.com/indigo-the-agent/aamas2024_submission709/2-ontology/ocra_plan.owl#hasNumberOfTasks">
        <rdfs:subPropertyOf rdf:resource="http://www.ontologydesignpatterns.org/ont/dul/DUL.owl#hasQuality"/>
        <owl:inverseOf rdf:resource="https://github.com/indigo-the-agent/aamas2024_submission709/2-ontology/ocra_plan.owl#isNumberOfTasksOf"/>
        <rdfs:domain rdf:resource="http://www.ontologydesignpatterns.org/ont/dul/DUL.owl#Plan"/>
        <rdfs:range rdf:resource="http://www.ontologydesignpatterns.org/ont/dul/DUL.owl#Quality"/>
        <rdfs:comment xml:lang="en">Relation between a Plan and the total number of tasks defined in the plan.

One might think that this relation could be modeled as a Data property instead of using an Object property. However, data instances cannot act as subjects in triples, thus, it would not be possible to represent some desirable statements such as &apos;the number of tasks of a plan is better/worse/equivalent to the number of tasks of a nother plan&apos;. For this reason, the relation is modeled as an Object property and users will need to add the actual value using the data property &apos;has data value&apos;.  

Example of use: Px (instance of Plan) &apos;has number of tasks&apos; Qx (instance of Quality) that &apos;has data value&apos; 1600. 

It is recomended to use an unsigned integer for the encoded data value, thus, the number of tasks might be zero but never lower than zero.</rdfs:comment>
        <rdfs:label xml:lang="en">has number of tasks</rdfs:label>
    </owl:ObjectProperty>
    


    <!-- https://github.com/indigo-the-agent/aamas2024_submission709/2-ontology/ocra_plan.owl#hasWorseQualityValueThan -->

    <owl:ObjectProperty rdf:about="https://github.com/indigo-the-agent/aamas2024_submission709/2-ontology/ocra_plan.owl#hasWorseQualityValueThan">
        <rdfs:subPropertyOf rdf:resource="http://www.ontologydesignpatterns.org/ont/dul/DUL.owl#associatedWith"/>
        <rdfs:domain rdf:resource="http://www.ontologydesignpatterns.org/ont/dul/DUL.owl#Quality"/>
        <rdfs:range rdf:resource="http://www.ontologydesignpatterns.org/ont/dul/DUL.owl#Quality"/>
        <rdfs:comment xml:lang="en">Relation between two Qualities that indicates that one of the qualities has a worse value than the other quality with respect to some criteria. 

Note that this ontology aims to model the result of comparing two qualities&apos; values, but it is out of the scope of the model to make any commitment regarding which is the criteria to compare the different values.</rdfs:comment>
        <rdfs:label xml:lang="en">has worse quality value than</rdfs:label>
    </owl:ObjectProperty>
    


    <!-- https://github.com/indigo-the-agent/aamas2024_submission709/2-ontology/ocra_plan.owl#isCheaperPlanThan -->

    <owl:ObjectProperty rdf:about="https://github.com/indigo-the-agent/aamas2024_submission709/2-ontology/ocra_plan.owl#isCheaperPlanThan">
        <rdfs:subPropertyOf rdf:resource="http://www.iri.upc.edu/groups/perception/OCRA/ont/ocra.owl#isBetterPlanThan"/>
        <owl:inverseOf rdf:resource="https://github.com/indigo-the-agent/aamas2024_submission709/2-ontology/ocra_plan.owl#isMoreExpensivePlanThan"/>
        <rdfs:domain rdf:resource="http://www.ontologydesignpatterns.org/ont/dul/DUL.owl#Plan"/>
        <rdfs:range rdf:resource="http://www.ontologydesignpatterns.org/ont/dul/DUL.owl#Plan"/>
        <owl:propertyDisjointWith rdf:resource="https://github.com/indigo-the-agent/aamas2024_submission709/2-ontology/ocra_plan.owl#isPlanWithSameCostAs"/>
        <rdfs:label xml:lang="en">is cheaper plan than</rdfs:label>
    </owl:ObjectProperty>
    


    <!-- https://github.com/indigo-the-agent/aamas2024_submission709/2-ontology/ocra_plan.owl#isCostOf -->

    <owl:ObjectProperty rdf:about="https://github.com/indigo-the-agent/aamas2024_submission709/2-ontology/ocra_plan.owl#isCostOf">
        <rdfs:subPropertyOf rdf:resource="http://www.ontologydesignpatterns.org/ont/dul/DUL.owl#isQualityOf"/>
        <rdfs:domain rdf:resource="http://www.ontologydesignpatterns.org/ont/dul/DUL.owl#Quality"/>
        <rdfs:range rdf:resource="http://www.ontologydesignpatterns.org/ont/dul/DUL.owl#Plan"/>
        <rdfs:comment xml:lang="en">For more information about this relation, please read the comment of its inverse &apos;has cost&apos;.</rdfs:comment>
        <rdfs:label xml:lang="en">is cost of</rdfs:label>
    </owl:ObjectProperty>
    


    <!-- https://github.com/indigo-the-agent/aamas2024_submission709/2-ontology/ocra_plan.owl#isEquivalentPlanTo -->

    <owl:ObjectProperty rdf:about="https://github.com/indigo-the-agent/aamas2024_submission709/2-ontology/ocra_plan.owl#isEquivalentPlanTo">
        <rdfs:subPropertyOf rdf:resource="http://www.ontologydesignpatterns.org/ont/dul/DUL.owl#associatedWith"/>
        <rdfs:label xml:lang="en">is equivalent plan to</rdfs:label>
    </owl:ObjectProperty>
    


    <!-- https://github.com/indigo-the-agent/aamas2024_submission709/2-ontology/ocra_plan.owl#isExpectedMakespanOf -->

    <owl:ObjectProperty rdf:about="https://github.com/indigo-the-agent/aamas2024_submission709/2-ontology/ocra_plan.owl#isExpectedMakespanOf">
        <rdfs:subPropertyOf rdf:resource="http://www.ontologydesignpatterns.org/ont/dul/DUL.owl#isQualityOf"/>
        <rdfs:domain rdf:resource="http://www.ontologydesignpatterns.org/ont/dul/DUL.owl#Quality"/>
        <rdfs:range rdf:resource="http://www.ontologydesignpatterns.org/ont/dul/DUL.owl#Plan"/>
        <rdfs:comment xml:lang="en">For more information about this relation, please read the comment of its inverse &apos;has expected makespan&apos;.</rdfs:comment>
        <rdfs:label xml:lang="en">is expected makespan of</rdfs:label>
    </owl:ObjectProperty>
    


    <!-- https://github.com/indigo-the-agent/aamas2024_submission709/2-ontology/ocra_plan.owl#isFasterPlanThan -->

    <owl:ObjectProperty rdf:about="https://github.com/indigo-the-agent/aamas2024_submission709/2-ontology/ocra_plan.owl#isFasterPlanThan">
        <rdfs:subPropertyOf rdf:resource="http://www.iri.upc.edu/groups/perception/OCRA/ont/ocra.owl#isBetterPlanThan"/>
        <owl:inverseOf rdf:resource="https://github.com/indigo-the-agent/aamas2024_submission709/2-ontology/ocra_plan.owl#isSlowerPlanThan"/>
        <rdfs:domain rdf:resource="http://www.ontologydesignpatterns.org/ont/dul/DUL.owl#Plan"/>
        <rdfs:range rdf:resource="http://www.ontologydesignpatterns.org/ont/dul/DUL.owl#Plan"/>
        <owl:propertyDisjointWith rdf:resource="https://github.com/indigo-the-agent/aamas2024_submission709/2-ontology/ocra_plan.owl#isPlanWithSameExpectedMakespanAs"/>
        <rdfs:label xml:lang="en">is faster plan than</rdfs:label>
    </owl:ObjectProperty>
    


    <!-- https://github.com/indigo-the-agent/aamas2024_submission709/2-ontology/ocra_plan.owl#isGraspedBy -->

    <owl:ObjectProperty rdf:about="https://github.com/indigo-the-agent/aamas2024_submission709/2-ontology/ocra_plan.owl#isGraspedBy">
        <rdfs:subPropertyOf rdf:resource="http://www.ontologydesignpatterns.org/ont/dul/DUL.owl#associatedWith"/>
        <rdfs:domain rdf:resource="http://www.ontologydesignpatterns.org/ont/dul/DUL.owl#PhysicalObject"/>
        <rdfs:range rdf:resource="http://www.ontologydesignpatterns.org/ont/dul/DUL.owl#Agent"/>
        <rdfs:comment xml:lang="en">Property to capture the relation between a physical object and the agent that grasps it. 

This relation is meant to be used for physical objects only, thus it is not considered the case of &apos;grasping and idea&apos;. For example, one might use this relation to represent the fact that a robot is grasping a piece of cloth.</rdfs:comment>
        <rdfs:label xml:lang="en">is grasped by</rdfs:label>
    </owl:ObjectProperty>
    


    <!-- https://github.com/indigo-the-agent/aamas2024_submission709/2-ontology/ocra_plan.owl#isLongerPlanThan -->

    <owl:ObjectProperty rdf:about="https://github.com/indigo-the-agent/aamas2024_submission709/2-ontology/ocra_plan.owl#isLongerPlanThan">
        <rdfs:subPropertyOf rdf:resource="http://www.iri.upc.edu/groups/perception/OCRA/ont/ocra.owl#isWorsePlanThan"/>
        <owl:inverseOf rdf:resource="https://github.com/indigo-the-agent/aamas2024_submission709/2-ontology/ocra_plan.owl#isShorterPlanThan"/>
        <rdfs:domain rdf:resource="http://www.ontologydesignpatterns.org/ont/dul/DUL.owl#Plan"/>
        <rdfs:range rdf:resource="http://www.ontologydesignpatterns.org/ont/dul/DUL.owl#Plan"/>
        <owl:propertyDisjointWith rdf:resource="https://github.com/indigo-the-agent/aamas2024_submission709/2-ontology/ocra_plan.owl#isPlanWithSameNumberOfTasksAs"/>
        <rdfs:label xml:lang="en">is longer plan than</rdfs:label>
    </owl:ObjectProperty>
    


    <!-- https://github.com/indigo-the-agent/aamas2024_submission709/2-ontology/ocra_plan.owl#isMoreExpensivePlanThan -->

    <owl:ObjectProperty rdf:about="https://github.com/indigo-the-agent/aamas2024_submission709/2-ontology/ocra_plan.owl#isMoreExpensivePlanThan">
        <rdfs:subPropertyOf rdf:resource="http://www.iri.upc.edu/groups/perception/OCRA/ont/ocra.owl#isWorsePlanThan"/>
        <rdfs:domain rdf:resource="http://www.ontologydesignpatterns.org/ont/dul/DUL.owl#Plan"/>
        <rdfs:range rdf:resource="http://www.ontologydesignpatterns.org/ont/dul/DUL.owl#Plan"/>
        <owl:propertyDisjointWith rdf:resource="https://github.com/indigo-the-agent/aamas2024_submission709/2-ontology/ocra_plan.owl#isPlanWithSameCostAs"/>
        <rdfs:label xml:lang="en">is more expensive plan than</rdfs:label>
    </owl:ObjectProperty>
    


    <!-- https://github.com/indigo-the-agent/aamas2024_submission709/2-ontology/ocra_plan.owl#isNumberOfTasksOf -->

    <owl:ObjectProperty rdf:about="https://github.com/indigo-the-agent/aamas2024_submission709/2-ontology/ocra_plan.owl#isNumberOfTasksOf">
        <rdfs:subPropertyOf rdf:resource="http://www.ontologydesignpatterns.org/ont/dul/DUL.owl#isQualityOf"/>
        <rdfs:domain rdf:resource="http://www.ontologydesignpatterns.org/ont/dul/DUL.owl#Quality"/>
        <rdfs:range rdf:resource="http://www.ontologydesignpatterns.org/ont/dul/DUL.owl#Plan"/>
        <rdfs:comment xml:lang="en">For more information about this relation, please read the comment of its inverse &apos;has number of tasks&apos;.</rdfs:comment>
        <rdfs:label xml:lang="en">is number of tasks of</rdfs:label>
    </owl:ObjectProperty>
    


    <!-- https://github.com/indigo-the-agent/aamas2024_submission709/2-ontology/ocra_plan.owl#isPlanWithSameCostAs -->

    <owl:ObjectProperty rdf:about="https://github.com/indigo-the-agent/aamas2024_submission709/2-ontology/ocra_plan.owl#isPlanWithSameCostAs">
        <rdfs:subPropertyOf rdf:resource="https://github.com/indigo-the-agent/aamas2024_submission709/2-ontology/ocra_plan.owl#isEquivalentPlanTo"/>
        <owl:inverseOf rdf:resource="https://github.com/indigo-the-agent/aamas2024_submission709/2-ontology/ocra_plan.owl#isPlanWithSameCostAs"/>
        <rdf:type rdf:resource="http://www.w3.org/2002/07/owl#SymmetricProperty"/>
        <rdfs:domain rdf:resource="http://www.ontologydesignpatterns.org/ont/dul/DUL.owl#Plan"/>
        <rdfs:range rdf:resource="http://www.ontologydesignpatterns.org/ont/dul/DUL.owl#Plan"/>
        <rdfs:label xml:lang="en">is plan with same cost as</rdfs:label>
    </owl:ObjectProperty>
    


    <!-- https://github.com/indigo-the-agent/aamas2024_submission709/2-ontology/ocra_plan.owl#isPlanWithSameExpectedMakespanAs -->

    <owl:ObjectProperty rdf:about="https://github.com/indigo-the-agent/aamas2024_submission709/2-ontology/ocra_plan.owl#isPlanWithSameExpectedMakespanAs">
        <rdfs:subPropertyOf rdf:resource="https://github.com/indigo-the-agent/aamas2024_submission709/2-ontology/ocra_plan.owl#isEquivalentPlanTo"/>
        <owl:inverseOf rdf:resource="https://github.com/indigo-the-agent/aamas2024_submission709/2-ontology/ocra_plan.owl#isPlanWithSameExpectedMakespanAs"/>
        <rdf:type rdf:resource="http://www.w3.org/2002/07/owl#SymmetricProperty"/>
        <rdfs:domain rdf:resource="http://www.ontologydesignpatterns.org/ont/dul/DUL.owl#Plan"/>
        <rdfs:range rdf:resource="http://www.ontologydesignpatterns.org/ont/dul/DUL.owl#Plan"/>
        <owl:propertyDisjointWith rdf:resource="https://github.com/indigo-the-agent/aamas2024_submission709/2-ontology/ocra_plan.owl#isSlowerPlanThan"/>
        <rdfs:label xml:lang="en">is plan with same expected makespan as</rdfs:label>
    </owl:ObjectProperty>
    


    <!-- https://github.com/indigo-the-agent/aamas2024_submission709/2-ontology/ocra_plan.owl#isPlanWithSameNumberOfTasksAs -->

    <owl:ObjectProperty rdf:about="https://github.com/indigo-the-agent/aamas2024_submission709/2-ontology/ocra_plan.owl#isPlanWithSameNumberOfTasksAs">
        <rdfs:subPropertyOf rdf:resource="https://github.com/indigo-the-agent/aamas2024_submission709/2-ontology/ocra_plan.owl#isEquivalentPlanTo"/>
        <owl:inverseOf rdf:resource="https://github.com/indigo-the-agent/aamas2024_submission709/2-ontology/ocra_plan.owl#isPlanWithSameNumberOfTasksAs"/>
        <rdf:type rdf:resource="http://www.w3.org/2002/07/owl#SymmetricProperty"/>
        <rdfs:domain rdf:resource="http://www.ontologydesignpatterns.org/ont/dul/DUL.owl#Plan"/>
        <rdfs:range rdf:resource="http://www.ontologydesignpatterns.org/ont/dul/DUL.owl#Plan"/>
        <owl:propertyDisjointWith rdf:resource="https://github.com/indigo-the-agent/aamas2024_submission709/2-ontology/ocra_plan.owl#isShorterPlanThan"/>
        <rdfs:label xml:lang="en">is plan with same number of tasks as</rdfs:label>
    </owl:ObjectProperty>
    


    <!-- https://github.com/indigo-the-agent/aamas2024_submission709/2-ontology/ocra_plan.owl#isShorterPlanThan -->

    <owl:ObjectProperty rdf:about="https://github.com/indigo-the-agent/aamas2024_submission709/2-ontology/ocra_plan.owl#isShorterPlanThan">
        <rdfs:subPropertyOf rdf:resource="http://www.iri.upc.edu/groups/perception/OCRA/ont/ocra.owl#isBetterPlanThan"/>
        <rdfs:domain rdf:resource="http://www.ontologydesignpatterns.org/ont/dul/DUL.owl#Plan"/>
        <rdfs:range rdf:resource="http://www.ontologydesignpatterns.org/ont/dul/DUL.owl#Plan"/>
        <rdfs:label xml:lang="en">is shorter plan than</rdfs:label>
    </owl:ObjectProperty>
    


    <!-- https://github.com/indigo-the-agent/aamas2024_submission709/2-ontology/ocra_plan.owl#isSlowerPlanThan -->

    <owl:ObjectProperty rdf:about="https://github.com/indigo-the-agent/aamas2024_submission709/2-ontology/ocra_plan.owl#isSlowerPlanThan">
        <rdfs:subPropertyOf rdf:resource="http://www.iri.upc.edu/groups/perception/OCRA/ont/ocra.owl#isWorsePlanThan"/>
        <rdfs:domain rdf:resource="http://www.ontologydesignpatterns.org/ont/dul/DUL.owl#Plan"/>
        <rdfs:range rdf:resource="http://www.ontologydesignpatterns.org/ont/dul/DUL.owl#Plan"/>
        <rdfs:label xml:lang="en">is slower plan than</rdfs:label>
    </owl:ObjectProperty>
    


    <!-- 
    ///////////////////////////////////////////////////////////////////////////////////////
    //
    // Classes
    //
    ///////////////////////////////////////////////////////////////////////////////////////
     -->

    


    <!-- https://github.com/indigo-the-agent/aamas2024_submission709/2-ontology/ocra_plan.owl#PlanCost -->

    <owl:Class rdf:about="https://github.com/indigo-the-agent/aamas2024_submission709/2-ontology/ocra_plan.owl#PlanCost">
        <owl:equivalentClass>
            <owl:Class>
                <owl:intersectionOf rdf:parseType="Collection">
                    <rdf:Description rdf:about="http://www.ontologydesignpatterns.org/ont/dul/DUL.owl#Quality"/>
                    <owl:Restriction>
                        <owl:onProperty rdf:resource="https://github.com/indigo-the-agent/aamas2024_submission709/2-ontology/ocra_plan.owl#isCostOf"/>
                        <owl:someValuesFrom rdf:resource="http://www.ontologydesignpatterns.org/ont/dul/DUL.owl#Plan"/>
                    </owl:Restriction>
                </owl:intersectionOf>
            </owl:Class>
        </owl:equivalentClass>
        <rdfs:subClassOf rdf:resource="http://www.ontologydesignpatterns.org/ont/dul/DUL.owl#Quality"/>
        <rdfs:subClassOf>
            <owl:Restriction>
                <owl:onProperty rdf:resource="https://github.com/indigo-the-agent/aamas2024_submission709/2-ontology/ocra_plan.owl#isCostOf"/>
                <owl:someValuesFrom rdf:resource="http://www.ontologydesignpatterns.org/ont/dul/DUL.owl#Plan"/>
            </owl:Restriction>
        </rdfs:subClassOf>
        <rdfs:comment xml:lang="en">A Quality of Plans capturing the cost of executing the plan&apos;s sequence of tasks.</rdfs:comment>
        <rdfs:label xml:lang="en">Plan cost</rdfs:label>
    </owl:Class>
    


    <!-- https://github.com/indigo-the-agent/aamas2024_submission709/2-ontology/ocra_plan.owl#PlanExpectedMakespan -->

    <owl:Class rdf:about="https://github.com/indigo-the-agent/aamas2024_submission709/2-ontology/ocra_plan.owl#PlanExpectedMakespan">
        <owl:equivalentClass>
            <owl:Class>
                <owl:intersectionOf rdf:parseType="Collection">
                    <rdf:Description rdf:about="http://www.ontologydesignpatterns.org/ont/dul/DUL.owl#Quality"/>
                    <owl:Restriction>
                        <owl:onProperty rdf:resource="https://github.com/indigo-the-agent/aamas2024_submission709/2-ontology/ocra_plan.owl#isNumberOfTasksOf"/>
                        <owl:someValuesFrom rdf:resource="http://www.ontologydesignpatterns.org/ont/dul/DUL.owl#Plan"/>
                    </owl:Restriction>
                </owl:intersectionOf>
            </owl:Class>
        </owl:equivalentClass>
        <rdfs:subClassOf rdf:resource="http://www.ontologydesignpatterns.org/ont/dul/DUL.owl#Quality"/>
        <rdfs:subClassOf>
            <owl:Restriction>
                <owl:onProperty rdf:resource="https://github.com/indigo-the-agent/aamas2024_submission709/2-ontology/ocra_plan.owl#isNumberOfTasksOf"/>
                <owl:someValuesFrom rdf:resource="http://www.ontologydesignpatterns.org/ont/dul/DUL.owl#Plan"/>
            </owl:Restriction>
        </rdfs:subClassOf>
        <rdfs:comment xml:lang="en">A Quality of Plans capturing the expected makespan or duration of executing the plan&apos;s sequence of tasks.</rdfs:comment>
        <rdfs:label xml:lang="en">Plan expected makespan</rdfs:label>
    </owl:Class>
    


    <!-- https://github.com/indigo-the-agent/aamas2024_submission709/2-ontology/ocra_plan.owl#PlanNumberOfTasks -->

    <owl:Class rdf:about="https://github.com/indigo-the-agent/aamas2024_submission709/2-ontology/ocra_plan.owl#PlanNumberOfTasks">
        <owl:equivalentClass>
            <owl:Class>
                <owl:intersectionOf rdf:parseType="Collection">
                    <rdf:Description rdf:about="http://www.ontologydesignpatterns.org/ont/dul/DUL.owl#Quality"/>
                    <owl:Restriction>
                        <owl:onProperty rdf:resource="https://github.com/indigo-the-agent/aamas2024_submission709/2-ontology/ocra_plan.owl#isExpectedMakespanOf"/>
                        <owl:someValuesFrom rdf:resource="http://www.ontologydesignpatterns.org/ont/dul/DUL.owl#Plan"/>
                    </owl:Restriction>
                </owl:intersectionOf>
            </owl:Class>
        </owl:equivalentClass>
        <rdfs:subClassOf rdf:resource="http://www.ontologydesignpatterns.org/ont/dul/DUL.owl#Quality"/>
        <rdfs:subClassOf>
            <owl:Restriction>
                <owl:onProperty rdf:resource="https://github.com/indigo-the-agent/aamas2024_submission709/2-ontology/ocra_plan.owl#isExpectedMakespanOf"/>
                <owl:someValuesFrom rdf:resource="http://www.ontologydesignpatterns.org/ont/dul/DUL.owl#Plan"/>
            </owl:Restriction>
        </rdfs:subClassOf>
        <rdfs:comment xml:lang="en">A Quality of Plans capturing the number of tasks included in the plan.</rdfs:comment>
        <rdfs:label xml:lang="en">Plan number of tasks</rdfs:label>
    </owl:Class>
    


    <!-- 
    ///////////////////////////////////////////////////////////////////////////////////////
    //
    // General axioms
    //
    ///////////////////////////////////////////////////////////////////////////////////////
     -->

    <rdf:Description>
        <rdf:type rdf:resource="http://www.w3.org/2002/07/owl#AllDisjointProperties"/>
        <owl:members rdf:parseType="Collection">
            <rdf:Description rdf:about="https://github.com/indigo-the-agent/aamas2024_submission709/2-ontology/ocra_plan.owl#hasBetterQualityValueThan"/>
            <rdf:Description rdf:about="https://github.com/indigo-the-agent/aamas2024_submission709/2-ontology/ocra_plan.owl#hasEquivalentQualityValueThan"/>
            <rdf:Description rdf:about="https://github.com/indigo-the-agent/aamas2024_submission709/2-ontology/ocra_plan.owl#hasWorseQualityValueThan"/>
        </owl:members>
    </rdf:Description>
</rdf:RDF>



<!-- Generated by the OWL API (version 4.5.6.2018-09-06T00:27:41Z) https://github.com/owlcs/owlapi -->

